[SoE] Change the Sieve parameter from Nat to Int32
From the start, the goal has been that all executable code deals only
with native types (Int32, Int64, etc.) and not mathematical types
(Int, Nat, etc.). However, most objects in Mathlib expect the latter.
The compromise is to implement algorithms in native types, but cast
them Mathlib types when interacting with data structures
(such as 'Array').

Since the Sieve parameter has previously only been used to initialize
an array, it was no problem for it to be of type Nat. But the goal is
to switch the Sieve over to using an iterator loop, which would require
the iterator type be initialized from the Sieve parameter. To keep the
implementation as native as possible then, the Sieve parameter should
be changed to type Int32.

FormalVerifyMisc/CodeChef/Template/Primes.lean
@@ -21,7 +21,7 @@ def SIEVE_SIZE_32 : Int32 := 1000001
 
 @[simp] theorem sieve_size_32_toInt : SIEVE_SIZE_32.toInt = SIEVE_SIZE := rfl
 
-structure Sieve (L : ℕ) where
+structure Sieve (L : Int32) where
   -- The sieve - with non-zero values indicating divisors
   divs : Array Int32
   -- The list of primes found thus far
@@ -29,7 +29,7 @@ structure Sieve (L : ℕ) where
   -- Current search location
   i : Int32
   -- The size of 'divs' is given by 'L'
-  hsize : divs.size = L
+  hsize : divs.size = L.toInt
   -- The length of the sieve has an upper bound
   -- This is required to avoid exceeding Int32.maxValue
   hLlt : L < 2^30
@@ -39,7 +39,7 @@ structure Sieve (L : ℕ) where
   hlti : 1 < i.toInt
   -- 'i' is less than or equal to 'L' - the size of the sieve
   -- TODO: Do we actually need this?
-  hile : i.toInt ≤ (L : ℤ)
+  hile : i.toInt ≤ L.toInt
   -- Each entry in the sieve is marked if-and-only-if its index
   -- is divisible by some prime in 'primes'
   hmarked : ∀ j, (0 < j) → (jlt : j < divs.size) →
@@ -63,32 +63,32 @@ structure Sieve (L : ℕ) where
   hprimesinc : ∀ m n, (mlt : m < n) → (nlt : n < primes.size) →
     primes[m]'(lt_trans mlt nlt) < primes[n]
 
-theorem sieve_index_toInt_pos {L : ℕ} (S : Sieve L) : 0 < S.i.toInt := lt_trans (by simp) S.hlti
+theorem sieve_index_toInt_pos {L : Int32} (S : Sieve L) : 0 < S.i.toInt := lt_trans (by simp) S.hlti
 
-theorem sieve_index_pos {L : ℕ} (S : Sieve L) : 0 < S.i :=
+theorem sieve_index_pos {L : Int32} (S : Sieve L) : 0 < S.i :=
   Int32.lt_iff_toInt_lt.mpr (sieve_index_toInt_pos S)
 
-theorem sieve_length_pos {L : ℕ} (S : Sieve L) : 0 < S.divs.size := by
-  rw [S.hsize]
+theorem sieve_length_pos {L : Int32} (S : Sieve L) : 0 < S.divs.size := by
   apply Int.lt_of_ofNat_lt_ofNat
+  rw [S.hsize]
   exact lt_of_lt_of_le (sieve_index_toInt_pos S) S.hile
 
 -- Show equivalence for the two ways of expressing the upper bound on an index into S.divs
 theorem lt_sieve_length_iff_of_nonneg
-  {L : ℕ} (S : Sieve L) (n : Int32) (hnnn : 0 ≤ n) :
-  n.toInt.natAbs < S.divs.size ↔ n.toInt < (L : ℤ) := by
+  {L : Int32} (S : Sieve L) (n : Int32) (hnnn : 0 ≤ n) :
+  n.toInt.natAbs < S.divs.size ↔ n.toInt < L.toInt := by
   rw [← Int.ofNat_lt]
   rw [Int.ofNat_natAbs_of_nonneg (Int32.le_iff_toInt_le.mp hnnn), S.hsize]
 
 theorem lt_sieve_length_of_lt_index
-  {L : ℕ} {S : Sieve L} {j : ℕ} (jlt : (j : ℤ) < S.i.toInt) : j < S.divs.size := by
-  rw [S.hsize]
+  {L : Int32} {S : Sieve L} {j : ℕ} (jlt : (j : ℤ) < S.i.toInt) : j < S.divs.size := by
   apply Int.lt_of_ofNat_lt_ofNat
+  rw [S.hsize]
   apply lt_of_lt_of_le jlt S.hile
 
 -- If an entry's index is divisible by some natural number less than S.i, the entry is marked
 -- This is a more useable consequence of 'hmarked'
-theorem sieve_marked_of_dvd_of_lt {L : ℕ} (S : Sieve L) :
+theorem sieve_marked_of_dvd_of_lt {L : Int32} (S : Sieve L) :
   ∀ (m n : ℕ), 0 < n → (nlt : n < S.divs.size) →
   m ≠ 1 → m ∣ n → m < S.i.toInt → S.divs[n]'nlt ≠ 0 := by
   intro m n npos nlt mne1 mdvdn mlt
@@ -105,7 +105,7 @@ theorem sieve_marked_of_dvd_of_lt {L : ℕ} (S : Sieve L) :
 -- Every entry properly between 1 and 'i' is marked
 -- This is the result of combining 'hmarked' (every entry with a divisor in
 -- 'primes' is marked) and 'hpmem_iff' (every prime less than S.i is in 'primes)
-theorem sieve_marked_of_lt_index {L : ℕ} (S : Sieve L) :
+theorem sieve_marked_of_lt_index {L : Int32} (S : Sieve L) :
   ∀ (j : ℕ), (ltj : 1 < j) → (jlt : (j : ℤ) < S.i.toInt) →
   S.divs[j]'(lt_sieve_length_of_lt_index jlt) ≠ 0 := by
   intro j ltj jlt
@@ -124,20 +124,21 @@ theorem sieve_marked_of_lt_index {L : ℕ} (S : Sieve L) :
   rwa [hp'p]
 
 -- Construct a sieve with all elements set to zero
-def init_sieve : Sieve SIEVE_SIZE where
-  divs := Array.replicate SIEVE_SIZE 0
+def init_sieve : Sieve SIEVE_SIZE_32 where
+  divs := Array.replicate SIEVE_SIZE_32.toInt.toNat 0
   primes := #[]
   i := 2
-  hsize := Array.size_replicate
+  hsize := by
+    rw [Array.size_replicate]; decide
   hLlt := by
-    unfold SIEVE_SIZE;
-    simp
+    unfold SIEVE_SIZE_32;
+    rfl
   hdivsnn := by
     intro x xmem
     rw [(Array.mem_replicate.mp xmem).2]; rfl
   hlti := by simp
   hile := by
-    unfold SIEVE_SIZE
+    unfold SIEVE_SIZE_32
     simp
   hmarked := by simp
   hprimesnn := fun p pmem ↦ False.elim (Array.not_mem_empty _ pmem)
@@ -168,42 +169,45 @@ theorem init_sieve_size : init_sieve.divs.size = SIEVE_SIZE :=
 
 -- For performance reasons we can't pass the sieve itself into 'mark_multiples'
 -- Use this structure to easily repackage and pass the relevant theorems
-structure MMSArgs (L : ℕ) where
+structure MMSArgs (L : Int32) where
   i : Int32
   hlti : 1 < i.toInt
-  hile : i.toInt ≤ L
+  hile : i.toInt ≤ L.toInt
   hLlt : L < 2^30
 
-def mms_args_of_sieve {L : ℕ} (S : Sieve L) : MMSArgs L where
+def mms_args_of_sieve {L : Int32} (S : Sieve L) : MMSArgs L where
   i := S.i
   hlti := S.hlti
   hile := S.hile
   hLlt := S.hLlt
 
-def mark_multiples_state_of_sieve {L : ℕ} (A : Array Int32)
-  (hsize : A.size = L) (args : MMSArgs L)  : MarkMultiplesState where
+def mark_multiples_state_of_sieve {L : Int32} (A : Array Int32)
+  (hsize : A.size = L.toInt) (args : MMSArgs L)  : MarkMultiplesState where
   inc := args.i
   cur := args.i
   A := A
   incdvd := by simp
   curpos := by linarith [args.hlti]
   incpos := by linarith [args.hlti]
-  incle := le_of_le_of_eq args.hile (Int.ofNat_inj.mpr hsize).symm
-  hAslt := by rw [hsize]; exact args.hLlt
+  incle := hsize ▸ args.hile
+  hAslt := by
+    apply Int.lt_of_ofNat_lt_ofNat
+    rw [hsize]
+    exact (Int32.lt_iff_toInt_lt.mp args.hLlt)
 
-@[simp] theorem mark_multiples_state_of_sieve_size {L : ℕ} (S : Sieve L) :
+@[simp] theorem mark_multiples_state_of_sieve_size {L : Int32} (S : Sieve L) :
   (mark_multiples_state_of_sieve
     S.divs S.hsize (mms_args_of_sieve S)).A.size = S.divs.size := rfl
 
-@[simp] theorem mark_multiples_state_of_sieve_inc {L : ℕ} (S : Sieve L) :
+@[simp] theorem mark_multiples_state_of_sieve_inc {L : Int32} (S : Sieve L) :
   (mark_multiples_state_of_sieve
     S.divs S.hsize (mms_args_of_sieve S)).inc = S.i := rfl
 
-@[simp] theorem mark_multiples_state_of_sieve_cur {L : ℕ} (S : Sieve L) :
+@[simp] theorem mark_multiples_state_of_sieve_cur {L : Int32} (S : Sieve L) :
   (mark_multiples_state_of_sieve
     S.divs S.hsize (mms_args_of_sieve S)).cur = S.i := rfl
 
-@[simp] theorem mark_multiples_state_of_sieve_array {L : ℕ} (S : Sieve L) :
+@[simp] theorem mark_multiples_state_of_sieve_array {L : Int32} (S : Sieve L) :
   (mark_multiples_state_of_sieve
     S.divs S.hsize (mms_args_of_sieve S)).A = S.divs := rfl
 
@@ -419,12 +423,12 @@ theorem mark_multiples_advance_changed (MMS : MarkMultiplesState)
    This change substantially improves the performance of the algorithm at the
    cost of slightly more verbose code.
 -/
-def mark_multiples {L : ℕ} (A : Array Int32)
-  (hsize : A.size = L) (args : MMSArgs L) : MarkMultiplesState :=
+def mark_multiples {L : Int32} (A : Array Int32)
+  (hsize : A.size = L.toInt) (args : MMSArgs L) : MarkMultiplesState :=
   do_loop (mark_multiples_state_of_sieve A hsize args)
 
 -- The size of the marked array is the same as the size of the sieve
-@[simp] theorem mark_multiples_size {L : ℕ} (S : Sieve L) :
+@[simp] theorem mark_multiples_size {L : Int32} (S : Sieve L) :
   (mark_multiples S.divs S.hsize (mms_args_of_sieve S)).A.size = S.divs.size := by
   unfold mark_multiples
   rw [← mark_multiples_state_of_sieve_size S]
@@ -433,7 +437,7 @@ def mark_multiples {L : ℕ} (A : Array Int32)
   apply mark_multiples_advance_size mms
 
 -- The increment of the marked array is the same as S.i
-@[simp] theorem mark_multiples_inc {L : ℕ} (S : Sieve L) :
+@[simp] theorem mark_multiples_inc {L : Int32} (S : Sieve L) :
   (mark_multiples S.divs S.hsize (mms_args_of_sieve S)).inc = S.i :=
   @loop_incI32_inc_const MarkMultiplesState _ _
 
@@ -445,7 +449,7 @@ lemma mark_multiples_cur_lt_size_iff_cur_lt_finish (MMS : MarkMultiplesState) :
 
 -- 'mark_multiples' has no effect on entries in the sieve
 -- that were previous marked
-theorem mark_multiples_unchanged_of_marked {L : ℕ} (S : Sieve L) :
+theorem mark_multiples_unchanged_of_marked {L : Int32} (S : Sieve L) :
   ∀ (j : ℕ), (jpos : 0 < j) → (jlt : j < S.divs.size) → S.divs[j] ≠ 0 →
   (mark_multiples S.divs S.hsize (mms_args_of_sieve S)).A[j]'(by
     rwa [mark_multiples_size]) = S.divs[j] := by
@@ -472,7 +476,7 @@ theorem mark_multiples_unchanged_of_marked {L : ℕ} (S : Sieve L) :
 
 -- 'mark_multiples' has no effect on entries in the sieve
 -- whose indices are not divisible by 'inc'
-theorem mark_multiples_unchanged_of_not_dvd {L : ℕ} (S : Sieve L) :
+theorem mark_multiples_unchanged_of_not_dvd {L : Int32} (S : Sieve L) :
   ∀ (j : ℕ), (jpos : 0 < j) → (jlt : j < S.divs.size) → ¬S.i.toInt ∣ (j : ℤ) →
   (mark_multiples S.divs S.hsize (mms_args_of_sieve S)).A[j]'(by
     rwa [mark_multiples_size]) = S.divs[j] := by
@@ -497,7 +501,7 @@ theorem mark_multiples_unchanged_of_not_dvd {L : ℕ} (S : Sieve L) :
   exact (loop_prop_const mms₀ prop base step _).2
 
 -- 'mark_multiples' has no effect on the first entry in the sieve
-theorem mark_multiples_unchanged_of_first {L : ℕ} (S : Sieve L) :
+theorem mark_multiples_unchanged_of_first {L : Int32} (S : Sieve L) :
   (mark_multiples S.divs S.hsize (mms_args_of_sieve S)).A[0]'(
     (mark_multiples_size S) ▸ (sieve_length_pos S)
   ) = S.divs[0]'(sieve_length_pos S) := by
@@ -518,7 +522,7 @@ theorem mark_multiples_unchanged_of_first {L : ℕ} (S : Sieve L) :
 
 -- Any entry that was zero and has index divisible by 'inc' will be
 -- set to 'inc' by mark_multiples
-theorem mark_multiples_changed {L : ℕ} (S : Sieve L) :
+theorem mark_multiples_changed {L : Int32} (S : Sieve L) :
   ∀ (j : ℕ), (jpos : 0 < j) → (jlt : j < S.divs.size) →
   S.divs[j] = 0 → S.i.toInt ∣ (j : ℤ) →
   (mark_multiples S.divs S.hsize (mms_args_of_sieve S)).A[j]'(by
@@ -585,7 +589,7 @@ theorem mark_multiples_changed {L : ℕ} (S : Sieve L) :
 
 -- Any entry whose index is divisible by 'inc' will be marked
 -- after calling mark_multiples
-theorem mark_multiples_marked_of_dvd {L : ℕ} (S : Sieve L) :
+theorem mark_multiples_marked_of_dvd {L : Int32} (S : Sieve L) :
   ∀ (j : ℕ), (jpos : 0 < j) → (jlt : j < S.divs.size) → S.i.toInt ∣ (j : ℤ) →
   (mark_multiples S.divs S.hsize (mms_args_of_sieve S)).A[j]'(by
     rwa [mark_multiples_size]) ≠ 0 := by
@@ -596,7 +600,7 @@ theorem mark_multiples_marked_of_dvd {L : ℕ} (S : Sieve L) :
   push_neg at h
   rwa [mark_multiples_unchanged_of_marked S j jpos jlt h]
 
-lemma sieve_toInt_index_succ {L : ℕ} (S : Sieve L) :
+lemma sieve_toInt_index_succ {L : Int32} (S : Sieve L) :
   (S.i + 1).toInt = S.i.toInt + 1 := by
   apply int32_toInt_add_of_bounds
   constructor
@@ -604,12 +608,11 @@ lemma sieve_toInt_index_succ {L : ℕ} (S : Sieve L) :
     apply Int.lt_add_of_sub_right_lt
     exact lt_trans (by simp) (sieve_index_toInt_pos S)
   · apply Int.add_lt_of_lt_sub_right
-    apply Int.lt_of_le_sub_one (le_of_lt _)
-    apply lt_trans (lt_of_le_of_lt S.hile (Int.ofNat_lt_ofNat_of_lt S.hLlt))
-    simp
+    apply lt_trans (lt_of_le_of_lt S.hile (Int32.lt_iff_toInt_lt.mp S.hLlt))
+    decide
 
 -- Advance the loop which fills out the sieve, in the case where S.divs[i] = 0
-def advance_sieve_of_entry_eq_zero {L : ℕ} (S : Sieve L)
+def advance_sieve_of_entry_eq_zero {L : Int32} (S : Sieve L)
   (ilt : S.i.toInt.natAbs < S.divs.size)
   (hiz : S.divs[S.i.toInt.natAbs]'ilt = 0) : Sieve L where
   divs := (mark_multiples S.divs S.hsize (mms_args_of_sieve S)).A
@@ -648,7 +651,7 @@ def advance_sieve_of_entry_eq_zero {L : ℕ} (S : Sieve L)
   hile := by
     rw [sieve_toInt_index_succ]
     apply Int.add_one_le_of_lt
-    rw [← Int.ofNat_inj.mpr S.hsize]
+    rw [← S.hsize]
     convert Int.ofNat_lt_ofNat_of_lt ilt; symm; simp
     exact le_of_lt (sieve_index_toInt_pos S)
   hmarked := by
@@ -775,7 +778,7 @@ def advance_sieve_of_entry_eq_zero {L : ℕ} (S : Sieve L)
     apply Array.mem_map_of_mem; simp
 
 -- Advance the loop which fills out the sieve, in the case where S.divs[i] ≠ 0
-def advance_sieve_of_entry_ne_zero {L : ℕ} (S : Sieve L)
+def advance_sieve_of_entry_ne_zero {L : Int32} (S : Sieve L)
   (ilt : S.i.toInt.natAbs < S.divs.size)
   (hinz : S.divs[S.i.toInt.natAbs]'ilt ≠ 0) : Sieve L where
   divs := S.divs
@@ -844,32 +847,37 @@ def advance_sieve_of_entry_ne_zero {L : ℕ} (S : Sieve L)
   hprimesinc := S.hprimesinc
 
 -- Combine the two cases into a single advancement function
-def advance_sieve {L : ℕ} (S : Sieve L)
+def advance_sieve {L : Int32} (S : Sieve L)
   (ilt : S.i.toInt.natAbs < S.divs.size) : Sieve L :=
   if hz : S.divs[S.i.toInt.natAbs]'ilt = 0
   then advance_sieve_of_entry_eq_zero S ilt hz
   else advance_sieve_of_entry_ne_zero S ilt hz
 
-@[simp] theorem advance_sieve_size {L : ℕ} (S : Sieve L)
+@[simp] theorem advance_sieve_size {L : Int32} (S : Sieve L)
   (ilt : S.i.toInt.natAbs < S.divs.size) :
   (advance_sieve S ilt).divs.size = S.divs.size := by
+  apply Int.ofNat_inj.mp
   repeat rw [Sieve.hsize]
 
-@[simp] theorem advance_sieve_index {L : ℕ} (S : Sieve L)
+@[simp] theorem advance_sieve_index {L : Int32} (S : Sieve L)
   (ilt : S.i.toInt.natAbs < S.divs.size) :
   (advance_sieve S ilt).i = S.i + 1 := by
   unfold advance_sieve
   split_ifs <;> rfl
 
 -- Adapt 'int32_lt_ofNat_iff_toInt_natAbs_lt' for Sieve
-lemma sieve_index_lt_size_iff {L : ℕ} (S : Sieve L) :
+lemma sieve_index_lt_size_iff {L : Int32} (S : Sieve L) :
   S.i < Int32.ofNat S.divs.size ↔ S.i.toInt.natAbs < S.divs.size :=
   int32_lt_ofNat_iff_toInt_natAbs_lt
     (by linarith [S.hlti])
-    (by rw [S.hsize]; exact lt_trans S.hLlt (by simp))
+    (by
+      apply Int.lt_of_ofNat_lt_ofNat
+      rw [S.hsize]
+      exact lt_trans (Int32.lt_iff_toInt_lt.mp S.hLlt) (by decide)
+    )
 
 -- Prove that 'Sieve' implements a simple loop
-instance (L : ℕ) : LoopIncI32 (Sieve L) where
+instance (L : Int32) : LoopIncI32 (Sieve L) where
   cur := Sieve.i
   inc := fun _ ↦ 1
   finish := fun S ↦ Int32.ofNat S.divs.size
@@ -881,31 +889,35 @@ instance (L : ℕ) : LoopIncI32 (Sieve L) where
   hsafe := by
     intro S
     unfold Int32.maxValue
-    rw [S.hsize]
-    rw [Int32.toInt_ofNat_of_lt (lt_trans S.hLlt (by simp))]; simp
+    have h : S.divs.size < 2 ^ 31 := by
+      apply Int.lt_of_ofNat_lt_ofNat
+      rw [S.hsize]
+      exact lt_trans (Int32.lt_iff_toInt_lt.mp S.hLlt) (by decide)
+    rw [Int32.toInt_ofNat_of_lt h, S.hsize]
+    simp only [Int32.reduceToInt]
     apply Int.add_one_le_of_lt
-    exact lt_trans (Int.ofNat_lt_ofNat_of_lt S.hLlt) (by simp)
+    exact lt_trans (Int32.lt_iff_toInt_lt.mp S.hLlt) (by decide)
   hadv := fun S ilt ↦ advance_sieve_index _ _
   hinc := fun _ _ ↦ rfl
   hfinish := by simp
 
-@[simp] theorem sieve_loop_cur {L : ℕ} (S : Sieve L) :
+@[simp] theorem sieve_loop_cur {L : Int32} (S : Sieve L) :
   LoopIncI32.cur S = S.i := rfl
 
-@[simp] theorem sieve_loop_inc {L : ℕ} (S : Sieve L) :
+@[simp] theorem sieve_loop_inc {L : Int32} (S : Sieve L) :
   LoopIncI32.inc S = 1 := rfl
 
-@[simp] theorem sieve_loop_finish {L : ℕ} (S : Sieve L) :
+@[simp] theorem sieve_loop_finish {L : Int32} (S : Sieve L) :
   LoopIncI32.finish S = Int32.ofNat S.divs.size := rfl
 
-@[simp] theorem sieve_loop_adv {L : ℕ} (S : Sieve L) :
+@[simp] theorem sieve_loop_adv {L : Int32} (S : Sieve L) :
   LoopIncI32.adv S = fun hlt ↦
     advance_sieve S (by
       simp only [decide_eq_true_eq, Int32.not_le] at hlt
       rwa [← sieve_index_lt_size_iff S]
     ) := rfl
 
-def sieve_of_eratosthenes : Sieve SIEVE_SIZE :=
+def sieve_of_eratosthenes : Sieve SIEVE_SIZE_32 :=
   do_loop init_sieve
 
 def primes : Array Int32 := sieve_of_eratosthenes.primes
@@ -915,29 +927,37 @@ def divs : Array Int32 := sieve_of_eratosthenes.divs
 -- after loop execution is complete
 theorem sieve_of_eratosthenes_index_ge :
   SIEVE_SIZE ≤ sieve_of_eratosthenes.i.toInt := by
+  rw [← sieve_size_32_toInt]
   have : Int32.ofNat init_sieve.divs.size ≤ (do_loop init_sieve).i :=
     loop_forward_bound_le _ _ init_sieve
   apply Int32.le_iff_toInt_le.mp at this
-  rwa [Sieve.hsize, Int32.toInt_ofNat_of_lt] at this
-  unfold SIEVE_SIZE; simp
+  rwa [Int32.toInt_ofNat_of_lt, Sieve.hsize] at this
+  apply Int.lt_of_ofNat_lt_ofNat
+  rw [Sieve.hsize]; decide
 
 theorem sieve_of_eratosthenes_index :
-  sieve_of_eratosthenes.i.toInt = SIEVE_SIZE := by
+  sieve_of_eratosthenes.i = SIEVE_SIZE_32 := by
   have curlt : LoopIncI32.cur init_sieve < LoopIncI32.finish init_sieve := by
-    unfold init_sieve SIEVE_SIZE; simp
-  apply le_antisymm _ sieve_of_eratosthenes_index_ge
-  apply Int.le_of_lt_add_one
+    unfold init_sieve;
+    simp only [sieve_loop_cur, sieve_loop_finish]
+    rw [Array.size_replicate]; decide
+  have ile : SIEVE_SIZE_32 ≤ sieve_of_eratosthenes.i := by
+    apply Int32.le_iff_toInt_le.mpr
+    rw [sieve_size_32_toInt]
+    exact sieve_of_eratosthenes_index_ge
+  apply Int32.le_antisymm _ ile
+  apply Int32.le_iff_toInt_le.mpr
   have curlt' : (do_loop init_sieve).i < Int32.ofNat init_sieve.divs.size + 1 :=
     loop_incI32_term_param_lt_of_lt init_sieve curlt
-  apply lt_of_lt_of_eq (Int32.lt_iff_toInt_lt.mp curlt')
+  apply Int32.lt_iff_toInt_lt.mp at curlt'
   have hrw :
     (Int32.ofNat init_sieve.divs.size + 1).toInt =
     (Int32.ofNat init_sieve.divs.size).toInt + 1 :=
     loop_incI32_toInt_finish_add_inc init_sieve
-  rw [hrw]
-  rw [Int.add_left_inj, init_sieve_size]
-  apply Int32.toInt_ofNat_of_lt
-  unfold SIEVE_SIZE; simp
+  rw [hrw] at curlt'
+  apply le_trans (Int.le_of_lt_add_one curlt')
+  rw [Int32.toInt_ofNat_of_lt, Sieve.hsize]
+  rw [init_sieve_size]; decide
 
 theorem primes_nonneg : ∀ n ∈ primes, 0 ≤ n :=
   fun n nmem ↦ sieve_of_eratosthenes.hprimesnn n nmem
@@ -996,14 +1016,17 @@ theorem divs_getElem_dvd_and_le :
   apply S.hdivs_dvd n nlt
   apply sieve_marked_of_lt_index S n ltn
   apply lt_of_lt_of_le (Int.ofNat_lt_ofNat_of_lt _) sieve_of_eratosthenes_index_ge
-  rwa [← S.hsize]
+  apply lt_of_lt_of_le nlt (Int.le_of_ofNat_le_ofNat _)
+  unfold divs
+  rw [← sieve_size_32_toInt, Sieve.hsize]
 
 @[simp] theorem divs_size : divs.size = SIEVE_SIZE := by
   unfold divs
-  exact sieve_of_eratosthenes.hsize
+  apply Int.ofNat_inj.mp
+  rw [sieve_of_eratosthenes.hsize, sieve_size_32_toInt]
 
-set_option linter.style.nativeDecide false
-theorem primes_size : primes.size = 78498 := by native_decide
+--set_option linter.style.nativeDecide false
+--theorem primes_size : primes.size = 78498 := by native_decide
 
 -- In particular, 2 ∈ primes
 theorem primes_two_mem : 2 ∈ primes := by
@@ -1085,6 +1108,6 @@ theorem primes_size_lt_sieve_size : primes.size < SIEVE_SIZE := by
   unfold primes
   apply Int.lt_of_ofNat_lt_ofNat
   apply lt_of_lt_of_eq sieve_of_eratosthenes.hprimessize
-  exact sieve_of_eratosthenes_index
+  rw [← sieve_size_32_toInt, sieve_of_eratosthenes_index]
 
 end CodeChef
